theories/TRAKHTENBROT/Sig_noeq.v
@@ -16,7 +16,7 @@ From Undecidability.Shared.Libs.DLW.Vec
   Require Import pos vec.
 
 From Undecidability.TRAKHTENBROT
-  Require Import notations utils fol_ops fo_sig fo_terms fo_logic fo_sat discrete.
+  Require Import notations utils fol_ops fo_sig fo_terms fo_logic fo_sat.
 
 Set Implicit Arguments.
 
@@ -55,371 +55,334 @@ Section remove_interpreted.
   Notation 𝕋 := (fol_term Σ).
   Notation 𝔽 := (fol_form Σ).
 
-  Notation "x ≡ y" := (@fol_atom Σ e (eq_rect_r _ (x##y##ø) H_ae)) (at level 59).
+  Notation "x ≡ y" := (@fol_atom Σ e (cast (x##y##ø) (eq_sym H_ae))) (at level 59).
 
   Section encode_congruence.
 
-  Variable (X : Type) (M : fo_model Σ X).
+    Variable (X : Type) (M : fo_model Σ X).
 
-  Notation "x ≈ y" := (fom_rels M e (eq_rect_r _ (x##y##ø) H_ae)).
+    Notation "x ≈ y" := (fom_rels M e (cast (x##y##ø) (eq_sym H_ae))).
 
-  Local Fact fol_sem_e x y φ : fol_sem M φ (x ≡ y) = fo_term_sem M φ x ≈ fo_term_sem M φ y.
-  Proof.
-    simpl; f_equal.
-    rewrite H_ae; unfold eq_rect_r; simpl; auto.
-  Qed.
+    Local Fact fol_sem_e x y φ : fol_sem M φ (x ≡ y) = fo_term_sem M φ x ≈ fo_term_sem M φ y.
+    Proof. simpl; f_equal; rewrite H_ae; simpl; auto. Qed.
 
-  Let fol_syms_e x y : fol_syms (x ≡ y) = fo_term_syms x ++ fo_term_syms y.
-  Proof.
-    simpl.
-    rewrite H_ae; unfold eq_rect_r; simpl; auto.
-    rewrite <- app_nil_end; auto.
-  Qed.
+    Let fol_syms_e x y : fol_syms (x ≡ y) = fo_term_syms x ++ fo_term_syms y.
+    Proof. simpl; rewrite H_ae; simpl; auto; rewrite <- app_nil_end; auto. Qed.
 
-  Let fol_rels_e x y : fol_rels (x ≡ y) = e::nil.
-  Proof. auto. Qed.
+    Let fol_rels_e x y : fol_rels (x ≡ y) = e::nil.
+    Proof. auto. Qed.
 
-  Local Definition fol_vec_equiv n := fol_vec_fa (vec_set_pos (fun p : pos n => £(pos2nat p+n) ≡ £(pos2nat p))).
+    Local Definition fol_vec_equiv n := fol_vec_fa (vec_set_pos (fun p : pos n => £(pos2nat p+n) ≡ £(pos2nat p))).
 
-  Local Fact fol_vec_equiv_syms n : incl (fol_syms (fol_vec_equiv n)) nil.
-  Proof. 
-    unfold fol_vec_equiv.
-    rewrite fol_syms_vec_fa.
-    intros x; rewrite in_flat_map.
-    intros (D & HD & H); revert H.
-    apply vec_list_inv in HD.
-    destruct HD as (p & ->). 
-    rew vec; rewrite fol_syms_e; simpl; tauto.
-  Qed.
+    Local Fact fol_vec_equiv_syms n : incl (fol_syms (fol_vec_equiv n)) nil.
+    Proof. 
+      unfold fol_vec_equiv.
+      rewrite fol_syms_vec_fa.
+      intros x; rewrite in_flat_map.
+      intros (D & HD & H); revert H.
+      apply vec_list_inv in HD.
+      destruct HD as (p & ->). 
+      rew vec; rewrite fol_syms_e; simpl; tauto.
+    Qed.
 
-  Local Fact fol_vec_equiv_rels n : incl (fol_rels (fol_vec_equiv n)) (e::nil).
-  Proof. 
-    unfold fol_vec_equiv.
-    rewrite fol_rels_vec_fa.
-    intros x; rewrite in_flat_map.
-    intros (D & HD & H); revert H.
-    apply vec_list_inv in HD.
-    destruct HD as (p & ->); rew vec.
-  Qed.
+    Local Fact fol_vec_equiv_rels n : incl (fol_rels (fol_vec_equiv n)) (e::nil).
+    Proof. 
+      unfold fol_vec_equiv.
+      rewrite fol_rels_vec_fa.
+      intros x; rewrite in_flat_map.
+      intros (D & HD & H); revert H.
+      apply vec_list_inv in HD.
+      destruct HD as (p & ->); rew vec.
+    Qed.
 
-  Local Fact fol_vec_equiv_sem n φ : 
+    Local Fact fol_vec_equiv_sem n φ : 
                 fol_sem M φ (fol_vec_equiv n)
             <-> (forall p : pos n, φ (pos2nat p+n) ≈ φ (pos2nat p)).
-  Proof.
-    unfold fol_vec_equiv.
-    rewrite fol_sem_vec_fa.
-    apply forall_equiv; intros p; rew vec.
-    rewrite fol_sem_e; simpl; tauto.
-  Qed.
-
-  Section congr_syms.
-
-    Variable (s : syms Σ).
-
-    Let n := ar_syms _ s.
-
-    Let A := fol_vec_equiv n.
-    Let f : 𝕋 := in_fot s (vec_set_pos (fun p => £(pos2nat p))).
-    Let g : 𝕋 := in_fot s (vec_set_pos (fun p => £(pos2nat p+n))).
-    Let B := g ≡ f.
-
-    Let HrA : incl (fol_syms A) nil.       Proof. apply fol_vec_equiv_syms. Qed.
-    Let HsA : incl (fol_rels A) (e::nil).  Proof. apply fol_vec_equiv_rels. Qed.
-
-    Let HrB : incl (fol_syms B) (s::nil).
     Proof.
-      unfold B; simpl.
-      rewrite H_ae; unfold eq_rect_r.
-      intros x; do 2 (simpl; rewrite in_app_iff).
-      do 2 rewrite in_concat_iff.
-      intros [ | [ (l & Hx & H) | [ | [ (l & Hx & H) | [] ] ] ] ]; try tauto; revert Hx;
+      unfold fol_vec_equiv.
+      rewrite fol_sem_vec_fa.
+      apply forall_equiv; intros p; rew vec.
+      rewrite fol_sem_e; simpl; tauto.
+    Qed.
+
+    Section congr_syms.
+
+      Variable (s : syms Σ).
+
+      Let n := ar_syms _ s.
+
+      Let A := fol_vec_equiv n.
+      Let f : 𝕋 := in_fot s (vec_set_pos (fun p => £(pos2nat p))).
+      Let g : 𝕋 := in_fot s (vec_set_pos (fun p => £(pos2nat p+n))).
+      Let B := g ≡ f.
+
+      Let HrA : incl (fol_syms A) nil.       Proof. apply fol_vec_equiv_syms. Qed.
+      Let HsA : incl (fol_rels A) (e::nil).  Proof. apply fol_vec_equiv_rels. Qed.
+
+      Let HrB : incl (fol_syms B) (s::nil).
+      Proof.
+        unfold B; simpl.
+        rewrite H_ae; unfold eq_rect_r.
+        intros x; do 2 (simpl; rewrite in_app_iff).
+        do 2 rewrite in_concat_iff.
+        intros [ | [ (l & Hx & H) | [ | [ (l & Hx & H) | [] ] ] ] ]; try tauto; revert Hx;
+          apply vec_list_inv in H; destruct H as (p & ->); rew vec.
+      Qed.
+
+      Let HsB : incl (fol_rels B) (e::nil).
+      Proof. simpl; cbv; tauto. Qed.
+
+      Local Definition congr_syms : 𝔽 := fol_mquant fol_fa n (fol_mquant fol_fa n (A ⤑  B)).
+
+      Local Fact congr_syms_syms : incl (fol_syms congr_syms) (s::nil).
+      Proof.
+        unfold congr_syms.
+        do 2 rewrite fol_syms_mquant.
+        rewrite fol_syms_bin.
+        apply incl_app; auto.
+        intros x Hx; destruct (HrA _ Hx).
+      Qed.
+
+      Local Fact congr_syms_rels : incl (fol_rels congr_syms) (e::nil).
+      Proof.
+        unfold congr_syms.
+        do 2 rewrite fol_rels_mquant.
+        rewrite fol_rels_bin.
+        apply incl_app; auto.
+      Qed.
+
+      Local Definition congr_syms_spec φ : 
+               fol_sem M φ congr_syms
+           <-> forall v w, (forall p, vec_pos v p ≈ vec_pos w p) -> fom_syms M s v ≈ fom_syms M s w.
+      Proof.
+        unfold congr_syms.
+        rewrite fol_sem_mforall.
+        apply forall_equiv; intros v.
+        rewrite fol_sem_mforall.
+        apply forall_equiv; intros w.
+        rewrite fol_sem_bin_fix.
+        apply (fol_bin_sem_ext fol_imp).
+        + unfold A; rewrite fol_vec_equiv_sem.
+          apply forall_equiv; intros p; rew vec; simpl.
+          apply fol_equiv_ext; repeat f_equal.
+          * rewrite env_vlift_fix1, env_vlift_fix0; auto.
+          * rewrite env_vlift_fix0; auto.
+        + unfold B.
+          rewrite fol_sem_e; simpl. 
+          apply fol_equiv_ext; repeat f_equal; 
+            apply vec_pos_ext; intros p; rew vec; rew fot.
+          * rewrite env_vlift_fix1, env_vlift_fix0; auto.
+          * rewrite env_vlift_fix0; auto.
+      Qed.
+
+    End congr_syms.
+
+    Section congr_rels.
+
+      Variable (r : rels Σ).
+
+      Let n := ar_rels _ r.
+
+      Let A := fol_vec_equiv n.
+      Let B := @fol_atom Σ r (vec_set_pos (fun p => £(pos2nat p))).
+      Let C := @fol_atom Σ r (vec_set_pos (fun p => £(pos2nat p+n))).
+
+      Let HsA : incl (fol_syms A) nil.       Proof. apply fol_vec_equiv_syms. Qed.
+      Let HrA : incl (fol_rels A) (e::nil).  Proof. apply fol_vec_equiv_rels. Qed.
+
+      Let HsB : incl (fol_syms B) nil.
+      Proof.
+        unfold B; simpl.
+        intros x; rewrite in_flat_map.
+        intros (t & H & Ht); revert Ht.
         apply vec_list_inv in H; destruct H as (p & ->); rew vec.
-    Qed.
+      Qed.
 
-    Let HsB : incl (fol_rels B) (e::nil).
-    Proof. simpl; cbv; tauto. Qed.
+      Let HrB : incl (fol_rels B) (r::nil).
+      Proof. simpl; cbv; tauto. Qed.
 
-    Definition congr_syms : 𝔽 := fol_mquant fol_fa n (fol_mquant fol_fa n (A ⤑  B)).
+      Let HsC : incl (fol_syms C) nil.
+      Proof. 
+        unfold C; simpl.
+        intros x; rewrite in_flat_map.
+        intros (t & Ht & H); revert H.
+        apply vec_list_inv in Ht.
+        destruct Ht as (p & ->); rew vec; simpl; tauto.
+      Qed.
 
-    Fact congr_syms_syms : incl (fol_syms congr_syms) (s::nil).
-    Proof.
-      unfold congr_syms.
-      do 2 rewrite fol_syms_mquant.
-      rewrite fol_syms_bin.
-      apply incl_app; auto.
-      intros x Hx; destruct (HrA _ Hx).
-    Qed.
+      Let HrC : incl (fol_rels C) (e::r::nil).
+      Proof. simpl; cbv; tauto. Qed.
 
-    Fact congr_syms_rels : incl (fol_rels congr_syms) (e::nil).
-    Proof.
-      unfold congr_syms.
-      do 2 rewrite fol_rels_mquant.
-      rewrite fol_rels_bin.
-      apply incl_app; auto.
-    Qed.
+      Local Definition congr_rels : 𝔽 := fol_mquant fol_fa n (fol_mquant fol_fa n (A ⤑  (C ↔ B))).
 
-    Definition congr_syms_spec φ : 
-             fol_sem M φ congr_syms
-         <-> forall v w, (forall p, vec_pos v p ≈ vec_pos w p) -> fom_syms M s v ≈ fom_syms M s w.
-    Proof.
-      unfold congr_syms.
-      rewrite fol_sem_mforall.
-      apply forall_equiv; intros v.
-      rewrite fol_sem_mforall.
-      apply forall_equiv; intros w.
-      rewrite fol_sem_bin_fix.
-      apply (fol_bin_sem_ext fol_imp).
-      + unfold A; rewrite fol_vec_equiv_sem.
-        apply forall_equiv; intros p; rew vec; simpl.
-        apply fol_equiv_ext; repeat f_equal.
-        * rewrite env_vlift_fix1, env_vlift_fix0; auto.
-        * rewrite env_vlift_fix0; auto.
-      + unfold B.
-        rewrite fol_sem_e; simpl. 
-        apply fol_equiv_ext; repeat f_equal; 
-          apply vec_pos_ext; intros p; rew vec; rew fot.
-        * rewrite env_vlift_fix1, env_vlift_fix0; auto.
-        * rewrite env_vlift_fix0; auto.
-    Qed.
+      Local Fact congr_rels_syms : incl (fol_syms congr_rels) nil.
+      Proof.
+        unfold congr_rels.
+        do 2 rewrite fol_syms_mquant.
+        repeat rewrite fol_syms_bin.
+        repeat (apply incl_app; auto).
+      Qed.
 
-  End congr_syms.
+      Local Fact congr_rels_rels : incl (fol_rels congr_rels) (e::r::nil).
+      Proof.
+        unfold congr_rels.
+        do 2 rewrite fol_rels_mquant.
+        repeat rewrite fol_rels_bin.
+        repeat (apply incl_app; auto).
+        intros x Hx; destruct (HrA _ Hx); try subst x; simpl; tauto.
+      Qed.
 
-  Section congr_rels.
-
-    Variable (r : rels Σ).
-
-    Let n := ar_rels _ r.
-
-    Let A := fol_vec_equiv n.
-    Let B := @fol_atom Σ r (vec_set_pos (fun p => £(pos2nat p))).
-    Let C := @fol_atom Σ r (vec_set_pos (fun p => £(pos2nat p+n))).
-
-    Let HsA : incl (fol_syms A) nil.       Proof. apply fol_vec_equiv_syms. Qed.
-    Let HrA : incl (fol_rels A) (e::nil).  Proof. apply fol_vec_equiv_rels. Qed.
-
-    Let HsB : incl (fol_syms B) nil.
-    Proof.
-      unfold B; simpl.
-      intros x; rewrite in_flat_map.
-      intros (t & H & Ht); revert Ht.
-      apply vec_list_inv in H; destruct H as (p & ->); rew vec.
-    Qed.
-
-    Let HrB : incl (fol_rels B) (r::nil).
-    Proof. simpl; cbv; tauto. Qed.
-
-    Let HsC : incl (fol_syms C) nil.
-    Proof. 
-      unfold C; simpl.
-      intros x; rewrite in_flat_map.
-      intros (t & Ht & H); revert H.
-      apply vec_list_inv in Ht.
-      destruct Ht as (p & ->); rew vec; simpl; tauto.
-    Qed.
-
-    Let HrC : incl (fol_rels C) (e::r::nil).
-    Proof. simpl; cbv; tauto. Qed.
-
-    Definition congr_rels : 𝔽 := fol_mquant fol_fa n (fol_mquant fol_fa n (A ⤑  (C ↔ B))).
-
-    Fact congr_rels_syms : incl (fol_syms congr_rels) nil.
-    Proof.
-      unfold congr_rels.
-      do 2 rewrite fol_syms_mquant.
-      repeat rewrite fol_syms_bin.
-      repeat (apply incl_app; auto).
-    Qed.
-
-    Fact congr_rels_rels : incl (fol_rels congr_rels) (e::r::nil).
-    Proof.
-      unfold congr_rels.
-      do 2 rewrite fol_rels_mquant.
-      repeat rewrite fol_rels_bin.
-      repeat (apply incl_app; auto).
-      intros x Hx; destruct (HrA _ Hx); try subst x; simpl; tauto.
-    Qed.
-
-    Definition congr_rels_spec φ : 
+      Local Definition congr_rels_spec φ : 
              fol_sem M φ congr_rels
          <-> forall v w, (forall p, vec_pos v p ≈ vec_pos w p) 
                       -> fom_rels M r v <-> fom_rels M r w.
+      Proof.
+        unfold congr_rels.
+        rewrite fol_sem_mforall.
+        apply forall_equiv; intros v.
+        rewrite fol_sem_mforall.
+        apply forall_equiv; intros w.
+        simpl fol_sem at 1.
+        apply (fol_bin_sem_ext fol_imp).
+        + unfold A; rewrite fol_vec_equiv_sem.
+          apply forall_equiv; intros p; rew vec; simpl.
+          apply fol_equiv_ext; repeat f_equal.
+          * rewrite env_vlift_fix1, env_vlift_fix0; auto.
+          * rewrite env_vlift_fix0; auto.
+        + apply fol_equiv_sem_ext; apply fol_equiv_ext; f_equal;
+            apply vec_pos_ext; intros p; rew vec; rew fot.
+          * rewrite env_vlift_fix1, env_vlift_fix0; auto.
+          * rewrite env_vlift_fix0; auto.
+      Qed.
+
+    End congr_rels.
+
+    Definition Σ_eq_congruent : 𝔽 :=
+        fol_lconj (map congr_syms ls) 
+      ⟑ fol_lconj (map congr_rels lr).
+
+    Fact Σ_eq_congruent_syms : incl (fol_syms Σ_eq_congruent) ls.
     Proof.
-      unfold congr_rels.
-      rewrite fol_sem_mforall.
-      apply forall_equiv; intros v.
-      rewrite fol_sem_mforall.
-      apply forall_equiv; intros w.
-      simpl fol_sem at 1.
-      apply (fol_bin_sem_ext fol_imp).
-      + unfold A; rewrite fol_vec_equiv_sem.
-        apply forall_equiv; intros p; rew vec; simpl.
-        apply fol_equiv_ext; repeat f_equal.
-        * rewrite env_vlift_fix1, env_vlift_fix0; auto.
-        * rewrite env_vlift_fix0; auto.
-      + apply fol_equiv_sem_ext; apply fol_equiv_ext; f_equal;
-          apply vec_pos_ext; intros p; rew vec; rew fot.
-        * rewrite env_vlift_fix1, env_vlift_fix0; auto.
-        * rewrite env_vlift_fix0; auto.
+      unfold Σ_eq_congruent.
+      rewrite fol_syms_bin.
+      repeat rewrite fol_syms_bigop; simpl.
+      repeat apply incl_app; try (cbv; tauto).
+      + intros s; rewrite in_flat_map.
+        intros (A & HA & H); revert HA H.
+        rewrite in_map_iff; intros (x & <- & Hx) H.
+        apply congr_syms_syms in H; revert H.
+        intros [ <- | [] ]; auto.
+      + intros r; rewrite in_flat_map.
+        intros (A & HA & H); revert HA H.
+        rewrite in_map_iff; intros (x & <- & Hx) H.
+        apply congr_rels_syms in H; revert H.
+        intros [].
     Qed.
 
-  End congr_rels.
+    Fact Σ_eq_congruent_rels : incl (fol_rels Σ_eq_congruent) lr.
+    Proof.
+      unfold Σ_eq_congruent.
+      rewrite fol_rels_bin.
+      repeat rewrite fol_rels_bigop; simpl.
+      repeat apply incl_app; try (cbv; tauto).
+      + intros s; rewrite in_flat_map.
+        intros (A & HA & H); revert HA H.
+        rewrite in_map_iff; intros (x & <- & Hx) H.
+        apply congr_syms_rels in H; revert H.
+        intros [ <- | [] ]; simpl; auto.
+      + intros x; simpl.
+        rewrite in_flat_map.
+        intros (A & HA & H); revert HA H.
+        rewrite in_map_iff; intros (y & <- & Hy) H.
+        apply congr_rels_rels in H; revert H.
+        intros [ | [ <- | [] ] ]; subst; auto.
+    Qed.
 
-  Definition Σ_eq_congruent : 𝔽 :=
-    fol_lconj (map congr_syms ls) ⟑ fol_lconj (map congr_rels lr).
+    (** Σ_eq_congruence_spec encodes that ≈ is a congruence wrt to all
+        the symbols in ls and lr *)
 
-  Fact Σ_eq_congruent_syms : incl (fol_syms Σ_eq_congruent) ls.
-  Proof.
-    unfold Σ_eq_congruent.
-    rewrite fol_syms_bin.
-    repeat rewrite fol_syms_bigop; simpl.
-    repeat apply incl_app; try (cbv; tauto).
-    + intros s; rewrite in_flat_map.
-      intros (A & HA & H); revert HA H.
-      rewrite in_map_iff; intros (x & <- & Hx) H.
-      apply congr_syms_syms in H; revert H.
-      intros [ <- | [] ]; auto.
-    + intros r; rewrite in_flat_map.
-      intros (A & HA & H); revert HA H.
-      rewrite in_map_iff; intros (x & <- & Hx) H.
-      apply congr_rels_syms in H; revert H.
-      intros [].
-  Qed.
-
-  Fact Σ_eq_congruent_rels : incl (fol_rels Σ_eq_congruent) lr.
-  Proof.
-    unfold Σ_eq_congruent.
-    rewrite fol_rels_bin.
-    repeat rewrite fol_rels_bigop; simpl.
-    repeat apply incl_app; try (cbv; tauto).
-    + intros s; rewrite in_flat_map.
-      intros (A & HA & H); revert HA H.
-      rewrite in_map_iff; intros (x & <- & Hx) H.
-      apply congr_syms_rels in H; revert H.
-      intros [ <- | [] ]; simpl; auto.
-    + intros x; simpl.
-      rewrite in_flat_map.
-      intros (A & HA & H); revert HA H.
-      rewrite in_map_iff; intros (y & <- & Hy) H.
-      apply congr_rels_rels in H; revert H.
-      intros [ | [ <- | [] ] ]; subst; auto.
-  Qed.
-
-  (** Σ_eq_congruence_spec encodes that ≈ is a congruence wrt to all
-      the symbols in ls and lr *)
-
-  Fact Σ_eq_congruent_spec φ :
+    Fact Σ_eq_congruent_spec φ :
           fol_sem M φ Σ_eq_congruent
       <-> (forall s, In s ls -> forall v w, (forall p, vec_pos v p ≈ vec_pos w p) 
                                           -> fom_syms M s v ≈ fom_syms M s w)
        /\ (forall r, In r lr -> forall v w, (forall p, vec_pos v p ≈ vec_pos w p) 
                                           -> fom_rels M r v <-> fom_rels M r w).
-  Proof.
-    unfold Σ_eq_congruent.
-    rewrite fol_sem_bin_fix.
-    do 2 rewrite fol_sem_lconj.
-    apply (fol_bin_sem_ext fol_conj).
-    + split.
-      * intros H s Hs.
-        apply (congr_syms_spec _ φ), H, in_map_iff.
-        exists s; auto.
-      * intros H f; rewrite in_map_iff.
-        intros (s & <- & Hs).
-        apply congr_syms_spec, H; auto.
-    + split.
-      * intros H r Hr.
-        apply (congr_rels_spec _ φ), H, in_map_iff.
-        exists r; auto.
-      * intros H f; rewrite in_map_iff.
-        intros (r & <- & Hr).
-        apply congr_rels_spec, H; auto.
-  Qed.
+    Proof.
+      unfold Σ_eq_congruent.
+      rewrite fol_sem_bin_fix.
+      do 2 rewrite fol_sem_lconj.
+      apply (fol_bin_sem_ext fol_conj).
+      + split.
+        * intros H s Hs.
+          apply (congr_syms_spec _ φ), H, in_map_iff.
+          exists s; auto.
+        * intros H f; rewrite in_map_iff.
+          intros (s & <- & Hs).
+          apply congr_syms_spec, H; auto.
+      + split.
+        * intros H r Hr.
+          apply (congr_rels_spec _ φ), H, in_map_iff.
+          exists r; auto.
+        * intros H f; rewrite in_map_iff.
+          intros (r & <- & Hr).
+          apply congr_rels_spec, H; auto.
+    Qed.
 
-  Definition Σ_eq_equivalence := 
-                           (∀(£0 ≡ £0)) 
-                         ⟑ (∀(∀(£1 ≡ £0 ⤑ £0 ≡ £1)))
-                         ⟑ (∀(∀(∀(£2 ≡ £1 ⤑ £1 ≡ £0 ⤑ £2 ≡ £0)))).
+    Definition Σ_eq_equivalence := 
+            (∀ £0 ≡ £0) 
+          ⟑ (∀∀ £1 ≡ £0 ⤑ £0 ≡ £1)
+          ⟑ (∀∀∀ £2 ≡ £1 ⤑ £1 ≡ £0 ⤑ £2 ≡ £0).
+
+    Local Fact Σ_eq_equivalence_syms : fol_syms Σ_eq_equivalence = nil.
+    Proof.
+      unfold Σ_eq_equivalence.
+      repeat (rewrite fol_syms_bin || rewrite fol_syms_quant).
+      repeat rewrite fol_syms_e; auto.
+    Qed.
+
+    Local Fact Σ_eq_equivalence_rels : incl (fol_rels Σ_eq_equivalence) (e::nil).
+    Proof. simpl; cbv; tauto. Qed.
   
-  Fact Σ_eq_equiv_spec φ : 
+    Fact Σ_eq_equiv_spec φ : 
            fol_sem M φ Σ_eq_equivalence
        <-> (forall x, x ≈ x)
         /\ (forall x y, x ≈ y -> y ≈ x)
         /\ (forall x y z, x ≈ y -> y ≈ z -> x ≈ z).
-  Proof.
-    unfold Σ_eq_equivalence.
-    repeat (rewrite fol_sem_bin_fix).
-    repeat apply fol_bin_sem_ext.
-    + rewrite fol_sem_quant_fix; apply forall_equiv; intro.
-      rewrite fol_sem_e; simpl; tauto.
-    + do 2 (rewrite fol_sem_quant_fix; apply forall_equiv; intro).
-      rewrite fol_sem_bin_fix.
-      do 2 rewrite fol_sem_e; simpl; tauto.
-    + do 3 (rewrite fol_sem_quant_fix; apply forall_equiv; intro).
-      do 2 rewrite fol_sem_bin_fix.
-      do 3 rewrite fol_sem_e; simpl; tauto.
-  Qed.
+    Proof.
+      unfold Σ_eq_equivalence.
+      repeat (rewrite fol_sem_bin_fix).
+      repeat apply fol_bin_sem_ext.
+      + rewrite fol_sem_quant_fix; apply forall_equiv; intro.
+        rewrite fol_sem_e; simpl; tauto.
+      + do 2 (rewrite fol_sem_quant_fix; apply forall_equiv; intro).
+        rewrite fol_sem_bin_fix.
+        do 2 rewrite fol_sem_e; simpl; tauto.
+      + do 3 (rewrite fol_sem_quant_fix; apply forall_equiv; intro).
+        do 2 rewrite fol_sem_bin_fix.
+        do 3 rewrite fol_sem_e; simpl; tauto.
+    Qed.
 
-  Fact Σ_eq_equivalence_syms : fol_syms Σ_eq_equivalence = nil.
-  Proof.
-    unfold Σ_eq_equivalence.
-    repeat (rewrite fol_syms_bin || rewrite fol_syms_quant).
-    repeat rewrite fol_syms_e; auto.
-  Qed.
+    Definition Σ_eq_congruence := 
+          Σ_eq_congruent 
+        ⟑ Σ_eq_equivalence.
 
-  Fact Σ_eq_equivalence_rels : incl (fol_rels Σ_eq_equivalence) (e::nil).
-  Proof. simpl; cbv; tauto. Qed.
+    Fact Σ_eq_congruence_syms : incl (fol_syms Σ_eq_congruence) ls.
+    Proof.
+      unfold Σ_eq_congruence.
+      rewrite fol_syms_bin, Σ_eq_equivalence_syms, <- app_nil_end.
+      apply Σ_eq_congruent_syms.
+    Qed.
 
-  Definition Σ_eq_congruence := Σ_eq_congruent ⟑ Σ_eq_equivalence.
-
-  Fact Σ_eq_congruence_syms : incl (fol_syms Σ_eq_congruence) ls.
-  Proof.
-    unfold Σ_eq_congruence.
-    rewrite fol_syms_bin, Σ_eq_equivalence_syms, <- app_nil_end.
-    apply Σ_eq_congruent_syms.
-  Qed.
-
-  Fact Σ_eq_congruence_rels : incl (fol_rels Σ_eq_congruence) lr.
-  Proof.
-    unfold Σ_eq_congruence.
-    rewrite fol_rels_bin.
-    apply incl_app.
-    + apply Σ_eq_congruent_rels.
-    + intros x Hx.
-      apply Σ_eq_equivalence_rels in Hx.
-      destruct Hx as [ | [] ]; subst; auto.
-  Qed.
-
-  Variable φ : nat -> X.
-
-  Hypothesis Xfin : finite_t X.
-  Hypothesis Mdec : fo_model_dec M.
-  Hypothesis eq_congr : fol_sem M φ Σ_eq_congruence.
-
-  Infix "~b" := (@fo_bisimilar Σ ls lr _ M) (at level 70, no associativity).
-
-  Fact eq_bisim x y : x ≈ y <-> x ~b y.
-  Proof.
-    split.
-    + destruct eq_congr as (H1 & H2).
-      apply Σ_eq_congruent_spec in H1.
-      apply Σ_eq_equiv_spec in H2.
-      rewrite <- fom_eq_fol_characterization; auto.
-      revert x y; apply fom_eq_incl.
-      intros x y H; split.
-      * intros s Hs v p.
-        apply H1; simpl; auto.
-        intros q; destruct (pos_eq_dec p q); rew vec; auto.
-        apply (proj1 H2).
-      * intros r' Hr v p; apply H1; auto.
-        intros q; destruct (pos_eq_dec p q); rew vec; auto.
-        apply (proj1 H2).
-    + intros H.
-      specialize (H (£1 ≡ £0) (fun n => match n with 0 => x | _ => y end)).
-      do 2 rewrite fol_sem_e in H; apply H.
-      * rewrite fol_syms_e; simpl; intros _ [].
-      * rewrite fol_rels_e; intros x' [ | [] ]; try subst x'; auto.
-      * apply proj2, Σ_eq_equiv_spec in eq_congr.
-        apply (proj1 eq_congr).
-  Qed.
+    Fact Σ_eq_congruence_rels : incl (fol_rels Σ_eq_congruence) lr.
+    Proof.
+      unfold Σ_eq_congruence.
+      rewrite fol_rels_bin.
+      apply incl_app.
+      + apply Σ_eq_congruent_rels.
+      + intros x Hx.
+        apply Σ_eq_equivalence_rels in Hx.
+        destruct Hx as [ | [] ]; subst; auto.
+    Qed.
 
   End encode_congruence.
 
@@ -429,8 +392,9 @@ Section remove_interpreted.
 
     Variable (A : 𝔽) (X : Type).
 
-    Theorem Σ_noeq_sound : fo_form_fin_dec_eq_SAT_in _ H_ae A X
-                        -> fo_form_fin_dec_SAT_in (Σ_noeq A) X.
+    Theorem Σ_noeq_sound : 
+               fo_form_fin_dec_eq_SAT_in _ H_ae A X
+            -> fo_form_fin_dec_SAT_in (Σ_noeq A) X.
     Proof.
       intros (M & H1 & H2 & HE & phi & H5).
       exists M, H1, H2, phi; unfold Σ_noeq.
@@ -457,28 +421,55 @@ Section remove_interpreted.
 
   Section completeness.
 
+    (* Not sure how to make this one work over infinite models 
+       Need some replacement for the quotient below *)
+
+    Hint Resolve finite_t_pos.
+
     Variable (A : 𝔽) 
              (HA1 : incl (fol_syms A) ls) 
-             (HA2 : incl (fol_rels A) lr). 
+             (HA2 : incl (fol_rels A) lr).
 
-    Theorem Σ_noeq_complete : fo_form_fin_dec_SAT (Σ_noeq A)
-                           -> fo_form_fin_dec_eq_SAT e H_ae A.
+    Theorem Σ_noeq_complete : 
+               fo_form_fin_dec_SAT (Σ_noeq A)
+            -> fo_form_fin_dec_eq_SAT e H_ae A.
     Proof.
-      intros (X & M & H1 & H2 & phi & H5 & H6).
-      destruct (fo_fin_model_discretize ls lr H1 H2)
-        as (n & Mn & Mdec & p & H).
-      assert (fol_sem Mn (fun n => p (phi n)) (Σ_eq_congruence)) as H5'.
-      { revert H5; apply fo_model_projection with (p := p).
-        + intros; auto.
-        + apply Σ_eq_congruence_syms.
-        + intros x Hx.
-          apply Σ_eq_congruence_rels in Hx; simpl; auto. }
-      generalize (eq_bisim (finite_t_pos _) Mdec H5'); intros H7.
-      exists (pos n), Mn, (finite_t_pos _), Mdec.
-      exists.
-      { intros x y; simpl; rewrite H7, H; tauto. } 
-      exists (fun n => p (phi n)).
-      revert H6; apply fo_model_projection with (p := p); auto.
+      intros (X & M & H1 & H2 & phi & (H5 & H6) & H3).
+      apply Σ_eq_congruent_spec in H5.
+      destruct H5 as (H4 & H5).
+      apply Σ_eq_equiv_spec in H6.
+      destruct H6 as (H6 & H7 & H8).
+      set (R x y := fom_rels M e (cast (x ## y ## ø) (eq_sym H_ae))).
+      destruct H1 as (lX & HlX).
+      destruct decidable_EQUIV_fin_quotient with (l := lX) (R := R)
+        as [ n cls repr G1 G2 ]; auto.
+      + intros; apply H2.
+      + intros x; exists x; split; auto; apply H6.
+      + exists (pos n).
+        set (Mn := Mk_fo_model Σ
+               (fun s v => cls (fom_syms M s (vec_map repr v)))
+               (fun r v => fom_rels M r (vec_map repr v))).
+        exists Mn.
+        exists; auto.
+        exists. { intros r v; apply H2. }
+        exists.
+        { intros p q.
+          unfold Mn; simpl.
+          rewrite cast_fun; simpl.
+          unfold R in G2; rewrite G2, !G1; tauto. }
+        exists (fun n => cls (phi n)).
+        revert H3.
+        apply fo_model_projection' with (i := cls) (j := repr) (ls := ls) (lr := lr); auto.
+        * intros s v Hs; simpl; apply G2.
+          rewrite vec_map_map; red.
+          apply H4; auto.
+          intros p; rew vec; apply G2.
+          rewrite G1; auto.
+        * intros r v Hr; simpl.
+          rewrite vec_map_map.
+          apply H5; auto.
+          intros p; rew vec; apply G2.
+          rewrite G1; auto.
     Qed.
 
   End completeness.
